\section*{Aufgabe 9}
\subsection*{a)}
$
F^T =
\begin{pmatrix}
6 & 1 & 4 \\
5 & 8 & 9 \\
3 & 2 & 7
\end{pmatrix}^T
$
\subsection*{b)}
$
D \cdot E =
\begin{pmatrix}
1 & 5 & 3 & -4 \\
1 & 3 & 2 & 2 \\
4 & 5 & -3 & 2 \\
4 & 2 & 7 & 1
\end{pmatrix}
\cdot
\begin{pmatrix}
2 & 3 & 5 & 1 \\
-2 & 1 & 4 & 2 \\
3 & 4 & 3 & 3 \\
-1 & 3 & 0 & 1
\end{pmatrix}
=
\begin{pmatrix}
2-10+9+4 & 3+5+12-12 & 5+20+9 & 1+10+9-4 \\
2-6+6-2 & 3+3+8+6 & 5+12+6 & 1+6+6+2 \\
8-10-9-2 & 12+5-12+6 & 20+20-9 & 4+10-9+2 \\
8-4+21+1 & 12+2+28+3 & 20+8+21 & 4+4+21+1
\end{pmatrix}
=
\begin{pmatrix}
5 & 8 & 34 & 16 \\
0 & 20 & 23 & 15 \\
-13 & 11 & 31 & 7 \\
24 & 45 & 49 & 30 \\
\end{pmatrix}
$\\
$
E \cdot D =
\begin{pmatrix}
2 & 3 & 5 & 1 \\
-2 & 1 & 4 & 2 \\
3 & 4 & 3 & 3 \\
-1 & 3 & 0 & 1
\end{pmatrix}
\cdot
\begin{pmatrix}
1 & 5 & 3 & -4 \\
1 & 3 & 2 & 2 \\
4 & 5 & -3 & 2 \\
4 & 2 & 7 & 1
\end{pmatrix}
\\=
\begin{pmatrix}
2+3+20+4 & 10+9+25+2 & 6+6-15+7 & -8+6+10+1 \\
-2+1+16+8 & -10+3+20+4 & -6+2-12+14 & 8+2+8+2 \\
3+4+12+12 & 15+12+15+6 & 9+8-9+21 & -12+8+6+3 \\
-1+3+4 & -5+9+2 & -3+6+7 & 4+6+1
\end{pmatrix}
=
\begin{pmatrix}
29 & 46 & 4 & 9 \\
23 & 17 & -2 & 20 \\
31 & 48 & 29 & 5 \\
6 & 6 & 10 & 11 \\
\end{pmatrix}
$
\subsection*{c)}
$
a =
\begin{pmatrix}
6 & 5 & 3 & 4 \\
1 & 8 & 2 & 2 \\
4 & 9 & 3 & 2 \\
4 & 9 & 7 & 1
\end{pmatrix}
\cdot
\begin{pmatrix}
4 \\
2 \\
3 \\
1
\end{pmatrix}
=
\begin{pmatrix}
24+10+9+4 \\
4+16+6+2 \\
16+18+9+2 \\
16+18+21+1
\end{pmatrix}
=
\begin{pmatrix}
47 \\
28 \\
45 \\
56
\end{pmatrix}
$\\
$
b =
\begin{pmatrix}
2 & 0 & 0 & 0 \\
0 & 1 & 0 & 0 \\
0 & 0 & 3 & 0 \\
0 & 0 & 0 & 1
\end{pmatrix}
\cdot
\begin{pmatrix}
x \\
y \\
z \\
1
\end{pmatrix}
=
\begin{pmatrix}
2x \\
y \\
3z \\
1
\end{pmatrix}
$\\
$
c =
\begin{pmatrix}
\alpha & 0 & 0 & 1 \\
0 & 0 & \beta & 0 \\
\gamma & 0 & 1 & \delta \\
0 & \zeta & 0 & \eta
\end{pmatrix}
\cdot
\begin{pmatrix}
x \\
y \\
z \\
1
\end{pmatrix}
=
\begin{pmatrix}
\alpha x+1 \\
\beta z \\
\gamma x+z+\delta \\
\zeta y+\eta
\end{pmatrix}
$
\subsection*{d)}
$det G = 48-5 = 43$\\
$det H = 16+18+10-60-(-6)-(-8) = 44-60+14 = 58-60 = -2$\\
$
det J = 2\cdot det
\begin{pmatrix}
3 & -2 & 2 \\
2 & 3 & -3 \\
1 & 2 & 2
\end{pmatrix}
- (-3) \cdot det
\begin{pmatrix}
1 & -2 & 2 \\
3 & 3 & -3 \\
4 & 2 & 2
\end{pmatrix}
+ 1 \cdot det
\begin{pmatrix}
1 & 3 & 2 \\
3 & 2 & -3 \\
4 & 1 & 2
\end{pmatrix}
-4 \cdot det
\begin{pmatrix}
1 & 3 & -2 \\
3 & 2 & 3 \\
4 & 1 & 2
\end{pmatrix}
= 2\cdot(18+6+8-6-(-8)-(-18))+3\cdot(6+24+12-24-(-12)-(-6))+1\cdot(4+(-36)+6-16-18-(-3))-4\cdot(4+36+(-6)-(-16)-18-3) = 2 \cdot 52 + 3 \cdot 36 + (-57) - 4 \cdot 29 = 104+108-57-116 = 39$
\subsection*{e)}
$
(K | I) =
\begin{pmatrix}
2 & 3 & | & 1 & 0 \\
-1 & 4 & | & 0 & 1
\end{pmatrix}$\\
switch rows $I$ and $II$\\\\
$=
\begin{pmatrix}
-1 & 4 & | & 0 & 1 \\
2 & 3 & | & 1 & 0
\end{pmatrix}$\\
row $I = I \cdot (-1)$\\\\
$=
\begin{pmatrix}
1 & -4 & | & 0 & -1 \\
2 & 3 & | & 1 & 0
\end{pmatrix}$\\
row $II = II - 2\cdot I$\\\\
$=
\begin{pmatrix}
1 & -4 & | & 0 & -1 \\
0 & 11 & | & 1 & 2
\end{pmatrix}$\\
row $II = II \cdot \frac{1}{11}$\\\\
$=
\begin{pmatrix}
1 & -4 & | & 0 & -1 \\
0 & 1 & | & \frac{1}{11} & \frac{2}{11}
\end{pmatrix}$\\
row $I = I + 4\cdot II$\\\\
$=
\begin{pmatrix}
1 & 0 & | & \frac{4}{11} & -\frac{3}{11} \\
0 & 1 & | & \frac{1}{11} & \frac{2}{11}
\end{pmatrix}\\
\rightarrow K^{-1} = \begin{pmatrix}
\frac{4}{11} & -\frac{3}{11} \\
\frac{1}{11} & \frac{2}{11}
\end{pmatrix}
$\\

\noindent$
(L | I ) =
\begin{pmatrix}
3 & 2 & 6 & | & 1 & 0 & 0 \\
1 & 1 & 3 & | & 0 & 1 & 0 \\
-3 & -2 & -5 & | & 0 & 0 & 1
\end{pmatrix}$\\
row $III = III + I$\\\\
$=
\begin{pmatrix}
3 & 2 & 6 & | & 1 & 0 & 0 \\
1 & 1 & 3 & | & 0 & 1 & 0 \\
0 & 0 & 1 & | & 1 & 0 & 1
\end{pmatrix}$\\
row $I = I - 2 \cdot II$\\\\
$=
\begin{pmatrix}
1 & 0 & 0 & | & 1 & -2 & 0 \\
1 & 1 & 3 & | & 0 & 1 & 0 \\
0 & 0 & 1 & | & 1 & 0 & 1
\end{pmatrix}$\\
row $II = II - I$\\\\
$=
\begin{pmatrix}
1 & 0 & 0 & | & 1 & -2 & 0 \\
0 & 1 & 3 & | & -1 & 3 & 0 \\
0 & 0 & 1 & | & 1 & 0 & 1
\end{pmatrix}$\\
row $II = II - 3 \cdot III$\\\\
$=
\begin{pmatrix}
1 & 0 & 0 & | & 1 & -2 & 0 \\
0 & 1 & 0 & | & -4 & 3 & -3 \\
0 & 0 & 1 & | & 1 & 0 & 1
\end{pmatrix}\\
\rightarrow L^{-1} =
\begin{pmatrix}
1 & -2 & 0 \\
-4 & 3 & -3 \\
1 & 0 & 1
\end{pmatrix}
$\\

\noindent$
(M | I ) =
\begin{pmatrix}
2 & -1 & 3 & 4 & | & 1 & 0 & 0 & 0 \\
1 & -2 & 0 & 2 & | & 0 & 1 & 0 & 0 \\
4 & -1 & 3 & 2 & | & 0 & 0 & 1 & 0 \\
0 & 1 & 2 & 1 & | & 0 & 0 & 0 & 1
\end{pmatrix}$\\
switch rows $I$ and $II$\\\\
$=
\begin{pmatrix}
1 & -2 & 0 & 2 & | & 0 & 1 & 0 & 0 \\
2 & -1 & 3 & 4 & | & 1 & 0 & 0 & 0 \\
4 & -1 & 3 & 2 & | & 0 & 0 & 1 & 0 \\
0 & 1 & 2 & 1 & | & 0 & 0 & 0 & 1
\end{pmatrix}$\\
row $II = II - 2\cdot I$\\
row $III = III - 4 \cdot I$\\\\
$=
\begin{pmatrix}
1 & -2 & 0 & 2 & | & 0 & 1 & 0 & 0 \\
0 & 3 & 3 & 0 & | & 1 & -2 & 0 & 0 \\
0 & 7 & 3 & -6 & | & 0 & -4 & 1 & 0 \\
0 & 1 & 2 & 1 & | & 0 & 0 & 0 & 1
\end{pmatrix}$\\
switch rows $II$ and $IV$\\\\
$=
\begin{pmatrix}
1 & -2 & 0 & 2 & | & 0 & 1 & 0 & 0 \\
0 & 1 & 2 & 1 & | & 0 & 0 & 0 & 1 \\
0 & 7 & 3 & -6 & | & 0 & -4 & 1 & 0 \\
0 & 3 & 3 & 0 & | & 1 & -2 & 0 & 0
\end{pmatrix}$\\
row $I = I + 2\cdot II$\\
row $III = III - 7\cdot II$\\
row $IV = IV - 3 \cdot II$\\\\
$=
\begin{pmatrix}
1 & 0 & 4 & 4 & | & 0 & 1 & 0 & 2 \\
0 & 1 & 2 & 1 & | & 0 & 0 & 0 & 1 \\
0 & 0 & -11 & -13 & | & 0 & -4 & 1 & -7 \\
0 & 0 & -3 & -3 & | & 1 & -2 & 0 & -3
\end{pmatrix}$\\
switch rows $III$ and $IV$\\\\
$=
\begin{pmatrix}
1 & 0 & 4 & 4 & | & 0 & 1 & 0 & 2 \\
0 & 1 & 2 & 1 & | & 0 & 0 & 0 & 1 \\
0 & 0 & -3 & -3 & | & 1 & -2 & 0 & -3 \\
0 & 0 & -11 & -13 & | & 0 & -4 & 1 & -7
\end{pmatrix}$\\
row $III = III \cdot -\frac{1}{3}$\\\\
$=
\begin{pmatrix}
1 & 0 & 4 & 4 & | & 0 & 1 & 0 & 2 \\
0 & 1 & 2 & 1 & | & 0 & 0 & 0 & 1 \\
0 & 0 & 1 & 1 & | & -\frac{1}{3} & \frac{2}{3} & 0 & 1 \\
0 & 0 & -11 & -13 & | & 0 & -4 & 1 & -7
\end{pmatrix}$\\
row $I = I - 4\cdot III$\\
row $II = II - 2\cdot III$\\
row $IV = IV + 11\cdot III$\\\\
$=
\begin{pmatrix}
1 & 0 & 0 & 0 & | & \frac{4}{3} & -\frac{5}{3} & 0 & -2 \\
0 & 1 & 0 & -1 & | & \frac{2}{3} & -\frac{4}{3} & 0 & -1 \\
0 & 0 & 1 & 1 & | & -\frac{1}{3} & \frac{2}{3} & 0 & 1 \\
0 & 0 & 0 & -2 & | & -\frac{11}{3} & \frac{10}{3} & 1 & 4
\end{pmatrix}$\\
row $IV = IV \cdot -\frac{1}{2}$\\\\
$=
\begin{pmatrix}
1 & 0 & 0 & 0 & | & \frac{4}{3} & -\frac{5}{3} & 0 & -2 \\
0 & 1 & 0 & -1 & | & \frac{2}{3} & -\frac{4}{3} & 0 & -1 \\
0 & 0 & 1 & 1 & | & -\frac{1}{3} & \frac{2}{3} & 0 & 1 \\
0 & 0 & 0 & 1 & | & \frac{11}{6} & -\frac{10}{6} & -\frac{1}{2} & -2
\end{pmatrix}$\\
row $II = II + IV$\\
row $III = III - IV$\\\\
$=
\begin{pmatrix}
1 & 0 & 0 & 0 & | & \frac{4}{3} & -\frac{5}{3} & 0 & -2 \\
0 & 1 & 0 & 0 & | & \frac{15}{6} & -\frac{18}{6} & -\frac{1}{2} & -3 \\
0 & 0 & 1 & 0 & | & -\frac{13}{6} & \frac{14}{6} & \frac{1}{2} & 3 \\
0 & 0 & 0 & 1 & | & \frac{11}{6} & -\frac{10}{6} & -\frac{1}{2} & -2
\end{pmatrix}
=
\begin{pmatrix}
1 & 0 & 0 & 0 & | & \frac{4}{3} & -\frac{5}{3} & 0 & -2 \\
0 & 1 & 0 & 0 & | & \frac{5}{2} & -3 & -\frac{1}{2} & -3 \\
0 & 0 & 1 & 0 & | & -\frac{13}{6} & \frac{7}{3} & \frac{1}{2} & 3 \\
0 & 0 & 0 & 1 & | & \frac{11}{6} & -\frac{5}{3} & -\frac{1}{2} & -2
\end{pmatrix}\\
\rightarrow M^{-1} = 
\begin{pmatrix}
1 & 0 & 0 & 0 & | & \frac{4}{3} & -\frac{5}{3} & 0 & -2 \\
0 & 1 & 0 & 0 & | & \frac{5}{2} & -3 & -\frac{1}{2} & -3 \\
0 & 0 & 1 & 0 & | & -\frac{13}{6} & \frac{7}{3} & \frac{1}{2} & 3 \\
0 & 0 & 0 & 1 & | & \frac{11}{6} & -\frac{5}{3} & -\frac{1}{2} & -2
\end{pmatrix}
$